CrMem.v
@@ -33,7 +33,7 @@ Inductive Instruction : Type :=
 | StOp (a1 a2 a3 : FnArg)
 | AddOp (dst a1 a2 : FnArg).
 
-Record MemProgram := {
+Record IM_Program := {
   fn_in : list (var_id * ValType);
   fn_body : list Instruction;
   fn_out_vars : list var_id;
@@ -48,6 +48,7 @@ Record machine_state {T : Type} := {
   tmp_map : PMap.t (TypedExpr T);
   iarr_map : PMap.t (TypedExpr T);
   varr_map : PMap.t (TypedExpr T);
+  bound_map : PMap.t (TypedExpr T);
   flag : HasError;
 }.
 Arguments machine_state T : clear implicits.
@@ -56,6 +57,7 @@ Definition set_io {T : Type} (m : machine_state T) (k : positive) (v : ValType *
   tmp_map := tmp_map m;
   iarr_map := iarr_map m;
   varr_map := varr_map m;
+  bound_map := bound_map m;
   flag := flag m;
 |}.
 Definition set_tmp {T : Type} (m : machine_state T) (k : positive) (v : ValType * T) := {|
@@ -63,6 +65,7 @@ Definition set_tmp {T : Type} (m : machine_state T) (k : positive) (v : ValType 
   tmp_map := PMap.set k v (tmp_map m);
   iarr_map := iarr_map m;
   varr_map := varr_map m;
+  bound_map := bound_map m;
   flag := flag m;
 |}.
 Definition set_iarr {T : Type} (m : machine_state T) (k : positive) (v : ValType * T) := {|
@@ -70,6 +73,7 @@ Definition set_iarr {T : Type} (m : machine_state T) (k : positive) (v : ValType
   tmp_map := tmp_map m;
   iarr_map := PMap.set k v (iarr_map m);
   varr_map := varr_map m;
+  bound_map := bound_map m;
   flag := flag m;
 |}.
 Definition set_varr {T : Type} (m : machine_state T) (k : positive) (v : ValType * T) := {|
@@ -77,6 +81,15 @@ Definition set_varr {T : Type} (m : machine_state T) (k : positive) (v : ValType
   tmp_map := tmp_map m;
   iarr_map := iarr_map m;
   varr_map := PMap.set k v (varr_map m);
+  bound_map := bound_map m;
+  flag := flag m;
+|}.
+Definition set_bound {T : Type} (m : machine_state T) (k : positive) (v : ValType * T) := {|
+  io_map := io_map m;
+  tmp_map := tmp_map m;
+  iarr_map := iarr_map m;
+  varr_map := varr_map m;
+  bound_map := PMap.set k v (bound_map m);
   flag := flag m;
 |}.
 Definition set_flag {T : Type} (m : machine_state T) (b : bool) := {|
@@ -84,6 +97,7 @@ Definition set_flag {T : Type} (m : machine_state T) (b : bool) := {|
   tmp_map := tmp_map m;
   iarr_map := iarr_map m;
   varr_map := varr_map m;
+  bound_map := bound_map m;
   flag := b;
 |}.
 
@@ -94,6 +108,7 @@ Inductive arith_expr :=
 | Z3_u32_var (name : positive)
 | Z3_bitadd (e1 e2 : arith_expr)
 | Z3_arr_ld (e1 : arr_expr) (e2 : arith_expr)
+| Z3_arith_max (e1 e2 : arith_expr)
 with ptr_expr :=
 | Z3_ptr_lit (x : uintptr)
 | Z3_ptr_var (name : positive)
@@ -112,6 +127,7 @@ Definition init_sym : sym_state := {|
   tmp_map := PMap.init (nil_t, Z3Nil);
   iarr_map := PMap.init (nil_t, Z3Nil);
   varr_map := PMap.init (nil_t, Z3Nil);
+  bound_map := PMap.init (nil_t, Z3Nil);
   flag := false;
 |}.
 
@@ -138,6 +154,7 @@ Definition apply_input (m : sym_state) (iv : list (positive * ValType)) : sym_st
   tmp_map := tmp_map init_sym;
   iarr_map := iarr_map init_sym;
   varr_map := apply_varr_helper (varr_map init_sym) iv;
+  bound_map := bound_map init_sym;
   flag := flag init_sym;
 |}.
 
@@ -184,49 +201,68 @@ Definition apply_sym_op (i : Instruction) (m : sym_state) : sym_state :=
       end
 
     | LdOp dst a1 a2 =>
-      let ld_val := match local_lookup a2 with
-      | (uint32_t, Z3Arith e2) =>
-        (* a2 is a valid index *)
-        let arr_a1 := match local_lookup a1 with
-        | (uintptr_t, Z3Ptr (Z3_ptr_lit x)) =>
+      let '(a1_t, a1_v) := local_lookup a1 in
+      let '(a2_t, a2_v) := local_lookup a2 in
+      match a1_t, a1_v, a2_t, a2_v with
+      | uintptr_t, Z3Ptr e1, int32_t, Z3Arith e2 =>
+        (* a1 is a pointer w/ value e1 *)
+        (* a2 is a uint32_t w/ value e2 *)
+        let lookup := match e1 with
+        | Z3_ptr_lit x =>
           (iarr_map m) !! (uptr_to_key x)
-        | (uintptr_t, Z3Ptr (Z3_ptr_var x)) =>
+        | Z3_ptr_var x =>
           (varr_map m) !! x
+        end in
+        let val := match lookup with
+        | (array_t, Z3Array A) => (uint8_t, Z3Arith (Z3_arr_ld A e2))
         | _ => (err_t, Z3Nil)
         end in
-        match arr_a1 with
-        | (array_t, Z3Array A) =>
-          (uint8_t, Z3Arith (Z3_arr_ld A e2))
-        | _ => (err_t, Z3Nil)
+        (* val is the value stored at a1[a2] *)
+        let m' := match e1 with 
+        | Z3_ptr_var x => match (bound_map m) !! x with
+          | (uint32_t, Z3Arith prev_bound) =>
+              set_bound m x (uint32_t, Z3Arith (Z3_arith_max e2 prev_bound))
+          | _ => set_bound m x (a2_t, a2_v)
+          end
+        | _ => m
+        end in
+        match val, dst with
+        | (uint8_t, Z3Arith _), IOArg x => set_io m' x val
+        | (uint8_t, Z3Arith _), TmpArg x => set_tmp m' x val
+        | _, _ => set_flag m true
         end
-      | _ => (err_t, Z3Nil)
-      end in
-      match ld_val, dst with
-      | (uint8_t, e3), IOArg x =>
-        set_io m x (uint8_t, e3)
-      | (uint8_t, e3), TmpArg x =>
-        set_tmp m x (uint8_t, e3)
-      | _, _ => set_flag m true
+      | _, _, _, _ => set_flag m true
       end
-
 
     | StOp a1 a2 a3 =>
       (* TODO: handle case where a1 is a ValArg imm_ptr *)
-      let arr_a1 :=
-      match local_lookup a1 with
-      | (uintptr_t, Z3Ptr (Z3_ptr_lit x)) =>
-        (array_t, (iarr_map m) !! (uptr_to_key x), set_iarr m (uptr_to_key x))
-      | (uintptr_t, Z3Ptr (Z3_ptr_var x)) =>
-        (array_t, (varr_map m) !! x, set_varr m x)
-      | (_, _) =>
-        (err_t, (err_t, Z3Arith (Z3_u8 (repr 0))), fun _ => m)
+      let st_idx := match local_lookup a2 with
+      | (uint32_t, Z3Arith e2) => (uint32_t, Z3Arith e2)
+      | _ => (err_t, Z3Nil)
       end in
-      match arr_a1, local_lookup a2, local_lookup a3 with
-      | (array_t, (array_t, Z3Array prev), setter), (uint32_t, Z3Arith e2), (uint8_t, Z3Arith e3) =>
-        setter (array_t, Z3Array (Z3_arr_st prev e2 e3))
+      let st_val := match local_lookup a3 with
+      | (uint8_t, Z3Arith e3) => (uint8_t, Z3Arith e3)
+      | _ => (err_t, Z3Nil)
+      end in
+      match local_lookup a1, st_idx, st_val with
+      | (uintptr_t, Z3Ptr (Z3_ptr_lit x)), (uint32_t, Z3Arith e2), (uint8_t, Z3Arith e3) =>
+        match (iarr_map m) !! (uptr_to_key x) with
+        | (array_t, Z3Array A) =>
+          set_iarr m (uptr_to_key x) (array_t, Z3Array (Z3_arr_st A e2 e3))
+        | _ => set_flag m true
+        end
+      | (uintptr_t, Z3Ptr (Z3_ptr_var x)), (uint32_t, Z3Arith e2), (uint8_t, Z3Arith e3) =>
+        match (varr_map m) !! x with
+        | (array_t, Z3Array A) =>
+          match (bound_map m) !! x with
+          | (uint32_t, Z3Arith prev_bound) =>
+              set_varr (set_bound m x (uint32_t, Z3Arith (Z3_arith_max e2 prev_bound))) x (array_t, Z3Array (Z3_arr_st A e2 e3))
+          | _ => set_varr (set_bound m x st_idx) x (array_t, Z3Array (Z3_arr_st A e2 e3))
+          end
+        | _ => set_flag m true
+        end
       | _, _, _ => set_flag m true
       end
-
 
     | AddOp dst a1 a2 =>
       let new_val : TypedExpr Z3Expr :=
@@ -250,19 +286,20 @@ Record output_valuation {T : Type} : Type := {
   var_val : var_id -> TypedExpr T;
   iptr_val : (uintptr * uint32) -> TypedExpr T;
   vptr_val : (var_id * uint32) -> TypedExpr T;
+  vptr_bound : var_id -> TypedExpr T;
 }.
 Arguments output_valuation T : clear implicits.
 
-Fixpoint compile_sym_helper (p : list Instruction) (m : sym_state) : sym_state :=
+Fixpoint sym_eval_helper (p : list Instruction) (m : sym_state) : sym_state :=
   match p with
   | [] => m
   | i :: rest =>
     let m' := apply_sym_op i m in
-    compile_sym_helper rest m'
+    sym_eval_helper rest m'
   end.
 
-Definition compile_sym (p : MemProgram) : output_valuation Z3Expr :=
-  let m' := compile_sym_helper (fn_body p) (apply_input init_sym (fn_in p)) in {|
+Definition sym_eval_program (p : IM_Program) : output_valuation Z3Expr :=
+  let m' := sym_eval_helper (fn_body p) (apply_input init_sym (fn_in p)) in {|
     errored := flag m';
     var_val := fun k => match (io_map m') !! k with
       | (nil_t, _) => (nil_t, Z3Nil)
@@ -276,7 +313,11 @@ Definition compile_sym (p : MemProgram) : output_valuation Z3Expr :=
     vptr_val := fun '(k, i) => match (varr_map m') !! k with
       | (array_t, Z3Array e) => (uint8_t, Z3Arith (Z3_arr_ld e (Z3_u32 i)))
       | _ => (err_t, Z3Nil)
-      end
+      end;
+    vptr_bound := fun k => match (bound_map m') !! k with
+      | (uint32_t, Z3Arith e) => (uint32_t, Z3Arith e)
+      | _ => (err_t, Z3Nil)
+      end;
   |}.
 
 Definition z3_s_val : Type := var_id -> CrVal.
@@ -308,6 +349,26 @@ Fixpoint eval_z3_arith (e : arith_expr) (sval : z3_s_val) (aval : z3_a_val) : Cr
     match res with
     | Legal v => v
     | Illegal => ErrorVal
+    end
+  | Z3_arith_max e1 e2 =>
+    let v1 := eval_z3_arith e1 sval aval in
+    let v2 := eval_z3_arith e2 sval aval in
+    match v1, v2 with
+    | IntVal (CrUInt8 x1), IntVal (CrUInt8 x2) =>
+      IntVal (CrUInt8 (
+        if (Integers.lt x1 x2) then
+          x2
+        else
+          x1
+      ))
+    | IntVal (CrUInt32 x1), IntVal (CrUInt32 x2) =>
+      IntVal (CrUInt32 (
+        if (Integers.lt x1 x2) then
+          x2
+        else
+          x1
+      ))
+    | _, _ => ErrorVal
     end
   end
 with eval_z3_array (e : arr_expr) (sval : z3_s_val) (aval : z3_a_val) : Array :=
@@ -348,9 +409,26 @@ Inductive Z3Bool :=
 | Z3_Disj (e1 e2 : Z3Bool)
 | Z3_Eq (e1 e2 : Z3Expr).
 
-Definition query_expression (p1 p2 : MemProgram) : Z3Bool :=
-  let val1 := compile_sym p1 in
-  let val2 := compile_sym p2 in
+(* Check that bounds are equal for all variable arrays *)
+Definition query_bounds (p1 p2 : IM_Program) : Z3Bool :=
+  let val1 := sym_eval_program p1 in
+  let val2 := sym_eval_program p2 in
+
+  (* Extract variable ids from input (uintptr_t) and output vaddrs *)
+  let input_vars := List.map fst (List.filter (fun '(_, t) => match t with uintptr_t => true | _ => false end) (fn_in p1)) in
+  let output_vars := List.map fst (fn_out_vaddrs p1) in
+  let bound_vars := input_vars ++ output_vars in
+
+  let b1 := List.map (vptr_bound val1) bound_vars in
+  let b2 := List.map (vptr_bound val2) bound_vars in
+  
+  fold_right Z3_Conj Z3_T
+    (map (fun '((_, x), (_, y)) => Z3_Eq x y) (combine b1 b2)).
+
+(* Check that outputs are equal (error flag, variables, and memory writes) *)
+Definition query_outputs (p1 p2 : IM_Program) : Z3Bool :=
+  let val1 := sym_eval_program p1 in
+  let val2 := sym_eval_program p2 in
 
   let o1 := (errored val1,
              List.map (var_val val1) (fn_out_vars p1),
@@ -373,11 +451,15 @@ Definition query_expression (p1 p2 : MemProgram) : Z3Bool :=
       (map (fun '((_, x), (_, y)) => Z3_Eq x y) (combine ip1 ip2)) in
     let vp_expr := fold_right Z3_Conj Z3_T
       (map (fun '((_, x), (_, y)) => Z3_Eq x y) (combine vp1 vp2)) in
-    Z3_Neg (Z3_Conj e_expr (
-            Z3_Conj v_expr (
-            Z3_Conj ip_expr
-                    vp_expr)))
+    Z3_Conj e_expr (
+    Z3_Conj v_expr (
+    Z3_Conj ip_expr
+            vp_expr))
   end.
+
+(* Main query: check if outputs and bounds differ *)
+Definition query_expression (p1 p2 : IM_Program) : Z3Bool :=
+  Z3_Neg (Z3_Conj (query_outputs p1 p2) (query_bounds p1 p2)).
 
 Inductive Z3Res :=
 | Z3Sat (s : z3_s_val) (a : z3_a_val)
@@ -407,21 +489,23 @@ Axiom z3_sound_none:
     z3_query e = Z3Unsat ->
     forall sval aval,
     eval_z3_bool e sval aval = false.
-    
+
+Definition matching_io (p1 p2 : IM_Program) : Prop :=
+  (fn_in p1) = (fn_in p2) /\
+  (fn_out_vars p1) = (fn_out_vars p2) /\
+  (fn_out_iaddrs p1) = (fn_out_iaddrs p2) /\
+  (fn_out_vaddrs p1) = (fn_out_vaddrs p2).
+
 Lemma mem_prog_soundness:
   (* for all programs, p1 and p2 *)
-  forall (p1 p2 : MemProgram),
-  (* with identical IO *)
-  (fn_in p1) = (fn_in p2) ->
-  (fn_out_vars p1) = (fn_out_vars p2) ->
-  (fn_out_iaddrs p1) = (fn_out_iaddrs p2) ->
-  (fn_out_vaddrs p1) = (fn_out_vaddrs p2) ->
+  forall (p1 p2 : IM_Program),
+  matching_io p1 p2 ->
   (* if z3 returns unsat *)
   z3_query (query_expression p1 p2) = Z3Unsat ->
   (* then under every possible valuation *)
   forall (sval : z3_s_val) (aval : z3_a_val),
-    let res1 := compile_sym p1 in
-    let res2 := compile_sym p2 in
+    let res1 := sym_eval_program p1 in
+    let res2 := sym_eval_program p2 in
     (* they have the same error value *)
     (errored res1 = errored res2) /\
     (* they have the same output variable assignments *)
@@ -446,4 +530,38 @@ Lemma mem_prog_soundness:
       eval_z3_expr x1 sval aval = eval_z3_expr x2 sval aval
     ).
 Proof.
+  intros p1 p2 Hio Hz3 sval aval res1 res2.
+  repeat split.
+  - admit.
+  - admit.
+  - admit.
 Admitted.
+
+Lemma mem_prog_completeness:
+  forall (p1 p2 : IM_Program) sval aval,
+  matching_io p1 p2 ->
+  (* if z3 returns sat *)
+  z3_query (query_expression p1 p2) = Z3Sat sval aval ->
+  (* at least one of the outputs differ under the sat valuation *)
+  let res1 := sym_eval_program p1 in
+  let res2 := sym_eval_program p2 in
+  (errored res1 <> errored res2) \/
+  (exists (v : var_id),
+    In v (fn_out_vars p1) /\
+    let '(_, x1) := (var_val res1) v in
+    let '(_, x2) := (var_val res2) v in
+    eval_z3_expr x1 sval aval <> eval_z3_expr x2 sval aval) \/
+  (exists (ia : uintptr) (ix1 : uint32),
+    In (ia, ix1) (fn_out_iaddrs p1) /\
+    let '(_, x1) := (iptr_val res1) (ia, ix1) in
+    let '(_, x2) := (iptr_val res2) (ia, ix1) in
+    eval_z3_expr x1 sval aval <> eval_z3_expr x2 sval aval) \/
+  (exists (va : var_id) (ix2 : uint32),
+    In (va, ix2) (fn_out_vaddrs p1) /\
+    let '(_, x1) := (vptr_val res1) (va, ix2) in
+    let '(_, x2) := (vptr_val res2) (va, ix2) in
+    eval_z3_expr x1 sval aval <> eval_z3_expr x2 sval aval).
+Proof.
+  intros p1 p2 sval aval Hio Hz3.
+Admitted.
+
